Interval.fst
@@ -1,9 +1,11 @@
 module Interval
 
 open ExtInt
+open FStar.List.Tot
+module G = FStar.GSet
 
 type interval = | EmptyInterval : interval
-		| SomeInterval  : (l:extInt) -> (r:extInt{l `lt` r}) -> interval
+		| SomeInterval  : (l:extInt) -> (r:extInt{l `le` r}) -> interval
 
 let mkExtInterval (l:extInt) (r:extInt{l `lt` r}) = SomeInterval l r
 let mkInterval (l:int) (r:int{l < r}) = SomeInterval (SomeInt l) (SomeInt r)
@@ -12,7 +14,11 @@ let union (a b:interval) = match a with
   | EmptyInterval -> b
   | SomeInterval l1 r1 -> match b with
 		 | EmptyInterval -> a
-		 | SomeInterval l2 r2 -> SomeInterval (min l1 l2) (max r1 r2) 
+		 | SomeInterval l2 r2 -> 
+                                assert (l1 `le` r1);
+                                assert (l2 `le` r2);
+                                assert (min l1 l2 `le` max r1 r2);
+                                SomeInterval (min l1 l2) (max r1 r2) 
 
 let inter (a b:interval) = match a with
   | SomeInterval l1 r1 -> 
@@ -24,13 +30,113 @@ let inter (a b:interval) = match a with
 	| _ -> b) // empty
   | _ -> a // if empty
 
+// [1; 3] is included in [0;4]
 let includes (a b:interval) = match a with
   | EmptyInterval -> true
   | SomeInterval l1 r1 -> match b with
     | EmptyInterval -> false
     | SomeInterval l2 r2 -> (l1 `ge` l2) && (r1 `le` r2)
 
-let gamma (i: interval) = match i with
-  | EmptyInterval -> fun _ -> False
-  | SomeInterval l r -> fun v' -> true == (let v = SomeInt v' in (v `ge` l) || (v `le` r))
-  
+
+
+let gamma (i: interval): GSet.set int = match i with
+  | EmptyInterval -> GSet.empty
+  | SomeInterval l r -> GSet.comprehend (fun v' -> let v = SomeInt v' in (v `ge` l) || (v `le` r))
+
+
+let lemma_includes_trans' (a:interval)
+                         (b:interval{includes a b})
+                         (c:interval{includes b c})
+                       : Lemma (includes a c) = ()
+                             
+let lemma_includes_trans (a:interval)
+                         (b:interval)
+                         (c: interval)
+                         : Lemma (includes a b ==> includes b c ==> includes a c) = ()
+                         // if includes a b && includes b c then (
+                         //   lemma_includes_trans' a b c
+                         // ) else ()
+
+
+let _ = assert (forall (a b c:interval). includes a b ==> includes b c ==> includes a c)
+let _ = assert (forall a b c. includes a b ==> includes b c ==> includes a c)
+
+let values_to_interval (l: list int) =
+  // let f #t (g:t->t->bool) (a:t) (b:t) : t = if a `g` b then a else b in
+  // let l = List.Tot.Base.map SomeInt lInt in
+  //             SomeInterval 
+  //                 (min minusInfty (fold_left (f lt) plusInfty l))
+  //                 (max plusInfty (fold_left (f gt) minusInfty l))
+  let enlarge (tup:extInt * extInt) (current':int) = (
+              let (l, r) = tup in
+              let current = SomeInt current' in
+              (min l current, max r current)
+            ) in
+  let (l, r) = fold_left enlarge (plusInfty, minusInfty) l in
+  if r `lt` l then EmptyInterval
+              else SomeInterval l r 
+
+let nonEmptyInterval = x:interval{SomeInterval? x}
+
+private
+let h1 (f:nonEmptyInterval -> nonEmptyInterval) (a:interval): interval = match a with
+  | EmptyInterval -> EmptyInterval
+  | _ -> f a
+
+private
+let h2 (f:nonEmptyInterval -> nonEmptyInterval -> nonEmptyInterval)
+       (a b:interval): interval = match a with
+  | EmptyInterval -> EmptyInterval
+  | _ -> match b with
+    | EmptyInterval -> EmptyInterval
+    | _ -> f a b
+
+let plus = h2 (fun a b ->
+    let (SomeInterval a1 a2) = a in
+    let (SomeInterval b1 b2) = b in
+    SomeInterval (a1 `plus` b1) (a2 `plus` b2)
+  )
+
+let minus = h2 (fun a b ->
+    let (SomeInterval a1 a2) = a in
+    let (SomeInterval b1 b2) = b in
+    SomeInterval (a1 `minus` b2) (a2 `minus` b1)
+  )
+
+let unaryMinus = h1 (fun a -> let (SomeInterval a1 a2) = a in
+                            SomeInterval (unaryMinus a2) (unaryMinus a1))
+
+let min4 (a, b, c, d) = min (min a b) (min c d) 
+let max4 (a, b, c, d) = max (max a b) (max c d) 
+let times = h2 (fun l r ->
+    let (SomeInterval a b) = l in
+    let (SomeInterval c d) = r in
+    let choices = (a `times` c, a `times` d, b `times` c, b `times` d) in
+    SomeInterval (min4 choices) (max4 choices)
+  )
+
+type maybe a = | Just : a -> maybe a | Nothing : maybe a
+
+let basic_le_interval_int (i:interval) (v':int) = match i with
+  | EmptyInterval -> Nothing
+  | SomeInterval a b -> let v = SomeInt v' in
+                       if a `le` v then Just (SomeInterval a (min b v))
+                       else             Nothing
+
+let basic_le_intervals (i j:interval) = match i with
+  | EmptyInterval -> Nothing
+  | SomeInterval a b -> match j with
+                       | EmptyInterval -> Nothing
+                       | SomeInterval c d -> if a `le` d then
+                                               Just (
+                                                 SomeInterval a (min b d),
+                                                 SomeInterval (max a c) d
+                                               )
+                                            else Nothing
+
+//Lemma (values_to_interval )
+
+// let rec lemma_includes_wide 
+//      (al ar bl br : extInt)
+//      (SomeInterval al ar:interval) (SomeInterval bl br:interval{includes a b})
+//      : Lemma (al `ge` )
