Main.fst
@@ -2,6 +2,7 @@ module Main
 
 open FStar.FunctionalExtensionality
 open FStar.GSet
+module CS = CSet
 open Interval
 open FStar.Tactics.Typeclasses
 open ExtInt
@@ -15,7 +16,7 @@ type lAExp =
   | LAExpMinus: lAExp -> lAExp -> lAExp 
   | LAExpMult : lAExp -> lAExp -> lAExp
 
-let ( +. ) = LAExpPlus 
+let ( +. ) = LAExpPlus
 let ( -. ) = LAExpMinus
 let ( *. ) = LAExpMult
 
@@ -81,16 +82,21 @@ let fib (max:int) =
     (i =. (!! i) +. (v 1))
   ) End)
 
-type state = string -> int
+type state (a:Type) = string -> a
 
-val emptyState : state
-let emptyState _ = 0
+class hasDefaultValue a = {
+  def: a
+}
+instance _ : hasDefaultValue int = {def = 0}
+
+let emptyState #a [| hasDefaultValue a |] () : state a =
+  fun _ -> def
 
 open FStar.Mul
 
 
 // interface _ : run_c = {} 
-val norm_lAExp : state -> lAExp -> int
+val norm_lAExp : state int -> lAExp -> int
 let rec norm_lAExp state exp =
   let fA a b g = g (norm_lAExp state a) (norm_lAExp state b) in
   match exp with 
@@ -100,7 +106,7 @@ let rec norm_lAExp state exp =
   | LAExpPlus a b -> fA a b  ( + )
   | LAExpVar v -> state v
 
-val norm_lBExp : state -> lBExp -> bool
+val norm_lBExp : state int -> lBExp -> bool
 let rec norm_lBExp state exp =
   let fA a b g = g (norm_lAExp state a) (norm_lAExp state b) in
   let fB a b g = g (norm_lBExp state a) (norm_lBExp state b) in
@@ -112,14 +118,13 @@ let rec norm_lBExp state exp =
   | LBExpOr a b -> fB a b ( || )
   | LBExpNot a -> norm_lBExp state a
 
-
 class run_c a b = {
-  run : state -> a -> b
+  run : state int -> a -> b
 }
 instance _ : run_c lAExp int = { run = norm_lAExp }
 instance _ : run_c lBExp bool = { run = norm_lBExp }
 
-val norm_lInstr : state -> lInstr -> (fuel:nat) -> Tot state (decreases fuel)
+val norm_lInstr : state int -> lInstr -> (fuel:nat) -> Tot (state int) (decreases fuel)
 let rec norm_lInstr state instr n = if n = 0 then state else
   let f = norm_lInstr in
   match instr with
@@ -131,17 +136,17 @@ let rec norm_lInstr state instr n = if n = 0 then state else
 				f state (b >> (while cond Do b End)) (n - 1)
 			  else  state
 
-instance _ : run_c lInstr state = { run = fun s a -> norm_lInstr s a 100 }
+instance _ : run_c lInstr (state int) = { run = fun s a -> norm_lInstr s a 100 }
 
-val execFib : int -> state
-let execFib n = (run emptyState (fib n))
+val execFib : int -> state int
+let execFib n = (run (emptyState ()) (fib n))
 
 let xx n = execFib n "a"
 
-let test = norm_lBExp emptyState (LBExpLitt true)
+let test = norm_lBExp (emptyState ()) (LBExpLitt true)
 
 
-let xxx = run emptyState (v 2 +. v 3)
+let xxx = run (emptyState ()) (v 2 +. v 3)
 
 let main = 
   let i = FStar.IO.input_int () in
@@ -161,7 +166,7 @@ let isPartialOrderL #a (cmp:a->a->Type0) (f:(a -> a -> Type0)) =
   /\ (forall a b  . f a b /\ f b a ==> cmp a b)
   /\ (forall a b c. f a b /\ f b c ==> f a c)
   
-class hasLPartialOrder a = {
+class hasLPartialOrder (a:Type) = {
   l_po_cmp : a -> a -> Type;
   l_po : (f:(a -> a -> Type){isPartialOrderL l_po_cmp f})
 }
@@ -175,125 +180,273 @@ instance _ : hasPartialOrder int = { po = fun a b -> a <= b }
 let isMonotonic #a #b [| hasLPartialOrder a |] [| hasLPartialOrder b |] (f:(a -> b)) =
   forall a b. a `l_po` b ==> f(a) `l_po` f(b)
 
-instance setLPO #c : hasLPartialOrder (set c) = {
- 	  l_po_cmp = equal;
-	  l_po = fun a b -> subset a b
+instance csetLPO #c : hasLPartialOrder (CSet.set c) = {
+ 	  l_po_cmp = CSet.equal;
+	  l_po = let h = (fun (a b: CSet.set c) -> true == CSet.subset a b) in admitP (isPartialOrderL CSet.equal h); h
  	}
 
-// val ssRefl : (#t:eqtype) -> (x: list t) -> Lemma (List.subset x x)
-// let rec ssRefl #t l = match l with
-//   | [] -> ()
-//   | h::tl -> assert (List.mem h l); admit (); ssRefl tl 
+instance gsetLPO #c : hasLPartialOrder (GSet.set c) = {
+ 	  l_po_cmp = GSet.equal;
+	  l_po = GSet.subset
+ 	}
 
-// let txtt (t:eqtype) = assert (forall (x: list t) . List.subset x x)
+// instance ordsetLPO (t:eqtype) (cmp:(t->t->bool){total_order t cmp}) : 
+// 	 hasLPartialOrder (ordset t cmp) = {
+//     l_po_cmp = equal
+//   ; l_po = fun a b -> subset a b
+// }
 
-// FStar.OrdSet.ordset
+let cset_to_set (#t:eqtype) (s:CSet.set t) =
+   GSet.as_set' (CSet.set_to_list s)
 
-open FStar.OrdSet
-
-instance ordsetLPO (t:eqtype) (cmp:(t->t->bool){total_order t cmp}) : 
-	 hasLPartialOrder (ordset t cmp) = {
-    l_po_cmp = equal
-  ; l_po = fun a b -> subset a b
-}
-
-let ord_to_set (#t:eqtype) (cmp:(t->t->bool){total_order t cmp}) (s:ordset t cmp) =
-  GSet.of_set (OrdSet.as_set s)
-
-class hasTotalOrder (a:eqtype) = {
-  to : (to:(a->a->bool){ total_order a to })
-}
-instance totImpPartial (a:eqtype) (_:hasTotalOrder a) : hasPartialOrder a = { po = to } 
+// class hasTotalOrder (a:eqtype) = {
+//   to : (to:(a->a->bool){ total_order a to })
+// }
+// instance totImpPartial (a:eqtype) (_:hasTotalOrder a) : hasPartialOrder a = { po = to } 
 
 class hasGaloisConnection (c:eqtype) a = {
-     c_to  : hasTotalOrder c
+     c_po  : hasPartialOrder c
    ; a_po  : hasPartialOrder a
    ; gamma : (f:(a -> set c){ isMonotonic f })
-   ; alpha : (f:(ordset c c_to.to -> a){ isMonotonic f })
-   ; galois_wf : (sa:a) -> (sc:ordset c to) ->
-		 Lemma (ord_to_set to sc `l_po` (gamma sa) /\ sa `l_po` (alpha sc))
+   ; alpha : (f:(CSet.set c -> a){ isMonotonic f })
+   ; galois_wf : (sa:a) -> (sc:CSet.set c) ->
+		 Lemma (cset_to_set sc `l_po` (gamma sa) /\ sa `l_po` (alpha sc))
 }
 
 let mkGaloisConnection (#c:eqtype) #a
-			     [| hasTotalOrder c   |]
+			     [| hasPartialOrder c   |]
 			     [| hasPartialOrder a |]
-			     (#to_c: hasTotalOrder c)
 			     (gamma:(a -> set c){ isMonotonic gamma })
-			     (alpha:(ordset c to_c.to -> a){ isMonotonic alpha })
-			     (galois_wf : (sa:a) -> (sc:ordset c to) -> 
-					Lemma (ord_to_set to sc `l_po` (gamma sa) /\ sa `l_po` (alpha sc))
+			     (alpha:(CSet.set c -> a){ isMonotonic alpha })
+			     (galois_wf : (sa:a) -> (sc:CSet.set c) -> 
+					Lemma (cset_to_set sc `l_po` (gamma sa) /\ sa `l_po` (alpha sc))
 			     )
   = {
-	c_to = to_c
-      ; a_po = solve
-      ; gamma = magic ()
-      ; alpha = magic ()
-      ; galois_wf = magic () //galois_wf
+	c_po      = solve
+      ; a_po      = solve
+      ; gamma     = gamma
+      ; alpha     = alpha
+      ; galois_wf = galois_wf
     }
+
+
 
 instance _ : hasPartialOrder interval = { po = includes }
 
-// instance _ : hasGaloisConnection int interval = mkGaloisConnection
-//    Interval.gamma
-//    (fun s -> )
+let interval_alpha set = Interval.values_to_interval (CSet.set_to_list set)
+let h l1 l2 = (l1 `l_po` l2 ==> interval_alpha l1 `po` interval_alpha l2)
+let _ = assert ( h [1;2;3] [1;3] )
 
-class abstractDomain c a = {
-  order : a -> a -> bool;
-  gamma : a -> (c -> Type0);
-  alpha : c -> a;
+open FStar.Tactics
+
+let rec lemma_intervalAlpha_eq_modulo_order (a:CSet.set int) (b:CSet.set int{CSet.equal a b})
+    : Lemma (interval_alpha a == interval_alpha b) = admit ()
+
+let rec inteval_alpha_behead_both (hd:int)
+                  (l1:CSet.set int{CSet.no_dup (hd::l1)})
+                  (l2:CSet.set int{CSet.no_dup (hd::l2)})
+      : Lemma (interval_alpha l1 `po` interval_alpha l2 == interval_alpha (hd::l1) `po` interval_alpha (hd::l2))
+      = match l1 with
+      | [] -> (match l2 with
+        | [] -> ()
+        | h2::t2 -> admit () 
+        )
+      | _ -> admit ()
+
+let rec lemma_intervalAlpha_ind (hd:int) (l1:CSet.set int{CSet.no_dup (hd::l1)})
+                  (l2:CSet.set int{CSet.mem hd l2 /\ interval_alpha l1 `po` interval_alpha (CSet.remove l2 hd)})
+    : Lemma (interval_alpha (hd::l1) `po` interval_alpha l2) = 
+            assert (CSet.no_dup (CSet.remove l2 hd));
+              
+            admitP (CSet.no_dup (hd::(CSet.remove l2 hd)));
+            admitP (CSet.equal l2 (hd::(CSet.remove l2 hd)));
+            assert (CSet.mem hd l2);
+            lemma_intervalAlpha_eq_modulo_order l2 (hd::(CSet.remove l2 hd));
+            inteval_alpha_behead_both hd l1 (CSet.remove l2 hd)
+
+let rec interval_alpha_monotonicy' (l1:CSet.set int) (l2:CSet.set int{l1 `l_po` l2})
+  : Lemma (interval_alpha l1 `po` interval_alpha l2)
+  = match l1 with
+  | [] -> ()
+  | hd::tl -> CSet.lemma_subset_remove tl l2 hd;
+            assert (CSet.subset tl (CSet.remove l2 hd));
+            assert (CSet.mem hd l2);
+            interval_alpha_monotonicy' tl (CSet.remove l2 hd);
+            assert (interval_alpha tl `po` interval_alpha (CSet.remove l2 hd));
+            lemma_intervalAlpha_ind hd tl l2
+
+let _ = assert (isMonotonic (Interval.gamma))
+
+instance _ : hasGaloisConnection int interval = mkGaloisConnection
+                                 Interval.gamma
+                                 (admitP (isMonotonic interval_alpha); interval_alpha)
+                                 (magic ())
+
+class hasAbstractDomain (c:eqtype) a = {
+  galois_connection : hasGaloisConnection c a;
   union : a -> a -> a;
   inter : a -> a -> a;
   bottom: a;
   top   : a;
   widen : a -> a -> a;
   assign: string -> a -> a;
-  op_eq : a -> a -> a
+  op_eq : a -> a -> a;
 }
 
-class test0 a = {
-  get0 : a -> int
+let mkAbstractDomain (#c:eqtype) #a
+                                  [| hasGaloisConnection c a |]
+                                  union inter bottom top widen assign op_eq
+    = {
+        galois_connection = solve
+      ; union = union
+      ; inter = inter
+      ; bottom = bottom
+      ; top = top
+      ; widen = widen
+      ; assign = assign
+      ; op_eq = op_eq
+    }
+
+class hasAbstractOperators (c:eqtype) a = {
+    abstract_domain:  hasAbstractDomain c a
+  ; default_value:    hasDefaultValue a
+  ; a_op_unary_minus: a -> a
+  ; a_op_unary_lift:  c -> a
+  ; a_op_plus:        a -> a -> a
+  ; a_op_minus:       a -> a -> a
+  ; a_op_times:       a -> a -> a
 }
 
-instance test0_int : test0 int = {get0 = (fun _ -> 10) }
+let mkAbstractOperators (#c:eqtype) #a [| hasAbstractDomain c a |] [| hasDefaultValue a |]
+  a_op_unary_minus a_op_plus a_op_minus a_op_times
+  = {
+    abstract_domain  = solve
+  ; default_value    = solve
+  ; a_op_unary_lift  = (fun c -> galois_connection.alpha (CSet.singleton c))
+  ; a_op_unary_minus = a_op_unary_minus
+  ; a_op_plus        = a_op_plus
+  ; a_op_minus       = a_op_minus
+  ; a_op_times       = a_op_times
+  }
 
-class test2 a = {
-  test0_super: test0 a;
-  get2: a -> int
+instance intervalDomain : hasAbstractDomain int interval = mkAbstractDomain
+                          Interval.union
+                          Interval.inter
+           (*bottom*)     Interval.EmptyInterval
+           (*top*)        (Interval.SomeInterval ExtInt.minusInfty ExtInt.plusInfty)
+           (*widen*)      Interval.union
+           (*assign*)     (fun _ i -> i)
+                          Interval.union
+
+instance _ : hasDefaultValue interval = {def = (SomeInterval (SomeInt 0) (SomeInt 0))}
+
+instance intervalOperators : hasAbstractOperators int interval = mkAbstractOperators
+                          Interval.unaryMinus
+                          Interval.plus
+                          Interval.minus
+                          Interval.times
+                          
+noeq
+type ctx (#c:eqtype) #a = {
+  memory: string -> state a
 }
 
-instance test0_eq (d : test2 'a) : test0 'a = d.test0_super
 
-let mktest2 (#a:Type) [| test0 a |] (f : a -> int)  = {
-  test0_super = solve;
-  get2 = f
+//let static_analysis_aexp (#c:eqtype{c==int}) #a [| hasAbstractOperators c a |]
+let rec static_analysis_aexp #a [| hasAbstractOperators int a |]
+                    (st:state a)
+                    (exp:lAExp)
+                    : a
+  = let rec h (exp:lAExp): a = 
+         match exp with
+       | LAExpLitt n       -> a_op_unary_lift n
+       | LAExpVar  varName -> st varName
+       | LAExpPlus a b     -> (h a) `a_op_plus` (h b)
+       | LAExpMinus a b    -> (h a) `a_op_minus` (h b)
+       | LAExpMult a b    ->  (h a) `a_op_times` (h b)
+    in h exp
+
+noeq
+type enumerableMap a = {
+   _em_data: string -> a
+ ; _em_keys: CSet.set string
 }
-
-instance _ : test2 int = mktest2 (fun z -> z * get0 z)
-
-let x = get2 22
-
-class test1 a (i:test0 a) = {
-  get1 : a -> int
+let state_to_em s = {_em_data = s;_em_keys = []}
+let em_get (m:enumerableMap 'a) (k:string): 'a = m._em_data k
+let em_set (m:enumerableMap 'a) (k:string) (v:'a) = let data = fun q -> if q = k then v else m._em_data q in {
+   _em_data = data
+ ; _em_keys = CSet.add_in_set k m._em_keys
 }
-
-instance hey (i:test0 'a) : test1 'a i = {
-  get1 = fun (x:'a) -> (get0 x) * 10
+let em_combine (m1 m2:enumerableMap 'a) (f:'a -> 'a -> 'a) = {
+   _em_data = (fun key -> f (em_get m1 key) (em_get m2 key))
+ ; _em_keys = CSet.union m2._em_keys m1._em_keys
 }
+let em_equal #a (myEq:a->a->bool) (m1 m2:enumerableMap a) =
+    let f1 = em_get m1 in
+    let f2 = em_get m2 in
+    let rec h l = (match l with
+      | [] -> true
+      | hd::tl -> if f1 hd `myEq` f2 hd then h tl else false  
+    ) in h (CSet.union m2._em_keys m1._em_keys)
 
-let asd = get1 1
+let rec interval_widen (i j:interval) = match (i, j) with
+  | (SomeInterval a b, SomeInterval c d) -> SomeInterval (if ExtInt.le a c then a else ExtInt.minusInfty)
+                                                        (if ExtInt.ge b d then b else ExtInt.plusInfty)
+  | (EmptyInterval, EmptyInterval) -> i
+  | (a, EmptyInterval) -> a
+  | (EmptyInterval, a) -> a
+
+//let rec em_bigger  
+
+let rec static_analysis_instr #a [| hasAbstractOperators int a |]// (#ad:hasAbstractDomain int a)
+                    (_inter: a -> a -> a) (*dirty hack*)
+                    (_eq: a -> a -> bool)
+                    (_w:  a -> a -> a)
+                    (st:enumerableMap a)
+                    (instr:lInstr)
+                    : Tot (enumerableMap a) (decreases instr)
+  = match instr with
+  | LInstrAssign name v -> em_set st name (static_analysis_aexp (em_get st) v)
+  | LInstrSkip -> st
+  | LInstrSeq b1 b2 -> static_analysis_instr _inter _eq _w (static_analysis_instr _inter _eq _w st b1) b2 
+  | LInstrIf c b1 b2 -> let r1 = static_analysis_instr _inter _eq _w st b1 in
+                       let r2 = static_analysis_instr _inter _eq _w st b2 in
+                       em_combine r1 r2 _inter
+  | LInstrWhile c b1 -> let execOnce st = static_analysis_instr _inter _eq _w st b1 in
+                       let rec lookForFixPoint st: Tot (enumerableMap a) = // (decreases (admitP (False))) = 
+                         let new_st  = execOnce st in
+                         let widened = em_combine st new_st _w in 
+                         if   em_equal _eq st widened
+                         then widened // new_st
+                         else lookForFixPoint new_st//(admitP (%[new_st] << %[st]); new_st)
+                       in execOnce st
+
+let myProg = (
+  (a =. (v 23)) >>
+  (a =. (!! a) +. (!! b))
+  )
+let myState : enumerableMap interval = 
+  em_set (state_to_em (emptyState ())) "b" (SomeInterval (SomeInt 2) (SomeInt 9))
 
 
-// interface _ : testx c a (abstractDomain) 
 
-let _ = mkabstractDomain
+let hey = static_analysis_instr Interval.inter (fun x y -> x = y) interval_widen myState myProg
 
-
-let aaa a b = a \/ b
-
-let asdasdxx = aaa True False
+let _ = assert (em_get hey "a" == magic()) by (compute (); qed ())
 
 
-let wellfounded #c #a (dom:abstractDomain c a) =
-  isPartialOrder dom.order
+let rec listToState (#a:Type) [| hasDefaultValue a |] (lst:list (tuple2 string a))
+  = fun (query:string) -> match lst with
+  | [] -> def
+  | (name, value)::tl -> if name = query then value else listToState tl query
 
+let test0 = static_analysis_aexp (listToState [
+  ("hey", SomeInterval (SomeInt 2) (SomeInt 4))
+]) (v 10 *. !! "hey")
 
+let _ = assert (test0 == magic ()) by (compute ();qed ())
+
+let verif_test0 = assert (test0 == SomeInterval (SomeInt 4) (SomeInt 4))
+
+//let hey =  static_analysis_aexp (emptyState ()) 
+//hey
